

CSC3310 Algorithms

Proof by Induction

William Retert

Milwaukee School of Engineering

Induction

Induction Proof technique for showing that some predicate is true for all positive integers.

Induction

Induction Proof technique for showing that some predicate is true for all positive integers.

Possible predicates $P(n)$:

- $\sum_{i=0}^n i = \frac{n(n+1)}{2}$
- $\sum_{i=0}^n 2^i = 2^{n+1} - 1$
- Peasant multiplication generates the correct result when multiplying an n -bit integer x by an integer y
- etc.

Basic steps:

- 1 Show $P(n)$ true for $n = 0$
- 2 Show that if $P(n)$ is true, then $P(n + 1)$ is also true.

Induction

Induction Proof technique for showing that some predicate is true for all positive integers.

Possible predicates $P(n)$:

- $\sum_{i=0}^n i = \frac{n(n+1)}{2}$
- $\sum_{i=0}^n 2^i = 2^{n+1} - 1$
- Peasant multiplication generates the correct result when multiplying an n -bit integer x by an integer y
- etc.

Basic steps:

- 1 Show $P(n)$ true for $n = 0$
- 2 Show that if $P(n - 1)$ is true, then $P(n)$ is also true.

Induction

Induction Proof technique for showing that some predicate is true for all positive integers.

Possible predicates $P(n)$:

- $\sum_{i=0}^n i = \frac{n(n+1)}{2}$
- $\sum_{i=0}^n 2^i = 2^{n+1} - 1$
- Peasant multiplication generates the correct result when multiplying an n -bit integer x by an integer y
- etc.

Basic steps:

- 1 Show $P(n)$ true for $n = 0$
- 2 Show that if $P(n - 1)$ is true, then $P(n)$ is also true.
Alternately, (strong induction), show that if $P(i)$ is true $\forall 1 \leq i < n$, then $P(n)$ is true

$$\sum_{i=1}^n i = \frac{n(n+1)}{2}$$

$$n = 0$$

$$\sum_{i=0}^0 i = 0 = \frac{0(1)}{2}$$

$$P(n-1) \vdash P(n)$$

$$\begin{aligned}\sum_{i=0}^n i &= n + \sum_{i=0}^{n-1} i \\ &= n + \frac{(n-1)((n-1)+1)}{2} \\ &= n + \frac{(n-1)n}{2} \\ &= \frac{2n}{2} + \frac{n^2 - n}{2} \\ &= \frac{n^2 + n}{2} \\ &= \frac{n(n+1)}{2}\end{aligned}$$

(Induction!)

$$\sum_{i=0}^n 2^i = 2^{n+1} - 1$$

$$n = 0$$

$$\sum_{i=0}^0 2^i = 2^0 = 1 = 2^1 - 1$$

$$P(n-1) \vdash P(n)$$

$$\begin{aligned}\sum_{i=0}^n 2^i &= 2^n + \sum_{i=0}^{n-1} 2^i \\ &= 2^n + (2^n - 1) && \text{(Induction!)} \\ &= 2 \cdot (2^n) - 1 \\ &= 2^{n+1} - 1\end{aligned}$$

“Peasant” Multiplication

Theorem

The “peasant” multiplication algorithm is correct. That is, for any n -bit integer x ,
 $\text{PEASANT}(x, y) = x \cdot y \quad \forall y \in \mathbb{Z}$

```
procedure PEASANT( $x, y$ )  
   $res \leftarrow 0$   
  while  $x > 0$  do  
    if  $x$  is odd then  
       $res \leftarrow res + y$   
    end if  
     $x \leftarrow \lfloor x \div 2 \rfloor$   
     $y \leftarrow y + y$   
  end while  
end procedure
```

We will rewrite the algorithm to be recursive in order to simplify the proof.

“Peasant” Multiplication

Theorem

The “peasant” multiplication algorithm is correct. That is, for any n -bit integer x ,
 $\text{PEASANT}(x, y) = x \cdot y \quad \forall y \in \mathbb{Z}$

```
procedure PEASANT( $x, y$ )  
   $res \leftarrow 0$   
  if  $x > 0$  then  
     $res \leftarrow \text{PEASANT}(\lfloor x \div 2 \rfloor, y + y)$   
    if  $x$  is odd then  
       $res \leftarrow res + y$   
    end if  
  end if  
  return  $res$   
end procedure
```

“Peasant” Multiplication

Theorem

The “peasant” multiplication algorithm is correct. That is, for any n -bit integer x ,
 $\text{PEASANT}(x, y) = x \cdot y \quad \forall y \in \mathbb{Z}$

```
procedure PEASANT( $x, y$ )  
   $res \leftarrow 0$   
  if  $x > 0$  then  
     $res \leftarrow \text{PEASANT}(\lfloor x \div 2 \rfloor, y + y)$   
    if  $x$  is odd then  
       $res \leftarrow res + y$   
    end if  
  end if  
  return  $res$   
end procedure
```

$n = 0$

If x has 0 bits, then $x = 0$,
and the algorithm correctly
computes $0 \times y = 0$

“Peasant” Multiplication

Theorem

The “peasant” multiplication algorithm is correct. That is, for any n -bit integer x ,
 $\text{PEASANT}(x, y) = x \cdot y \quad \forall y \in \mathbb{Z}$

$$P(n-1) \vdash P(n)$$

If x is a n -bit number, then $\lfloor x \div 2 \rfloor$ is an $(n-1)$ bit number. Therefore, by induction,

$$\text{PEASANT}(\lfloor x \div 2 \rfloor, y + y) = (\lfloor x \div 2 \rfloor) \times (y + y)$$

If x is even, our return value is then

$$\frac{x}{2} \times (2y) = x \cdot y$$

. If x is odd, the return value is

$$\begin{aligned} \frac{x-1}{2} \times (2y) + y &= (x-1)y + y \\ &= x \cdot y - y + y \\ &= x \cdot y \end{aligned}$$

```

procedure PEASANT(x,y)
  res  $\leftarrow$  0
  if x > 0 then
    res  $\leftarrow$  PEASANT( $\lfloor x \div 2 \rfloor$ , y+y)
    if x is odd then
      res  $\leftarrow$  res + y
    end if
  end if
  return res
end procedure

```